src/program_proof/tulip/program/replica/replica_repr.v
@@ -2,6 +2,7 @@ From Perennial.program_proof.tulip.program Require Import prelude.
 From Perennial.program_proof.tulip.program.tuple Require Import res.
 From Perennial.program_proof.tulip.program.txnlog Require Import txnlog.
 From Perennial.program_proof.tulip.program.index Require Import index.
+From Perennial.program_proof.tulip.paxos Require Import prelude.
 
 Section repr.
   Context `{!heapGS Σ, !tulip_ghostG Σ}.
@@ -130,11 +131,6 @@ Section repr.
       "Hlsna"      ∷ rp ↦[Replica :: "lsna"] #lsna ∗
       "%Hlencloga" ∷ ⌜length cloga = uint.nat lsna⌝.
 
-  Definition is_replica_txnlog (rp : loc) gid γ : iProp Σ :=
-    ∃ (txnlog : loc),
-      "#HtxnlogP" ∷ readonly (rp ↦[Replica :: "txnlog"] #txnlog) ∗
-      "#Htxnlog"  ∷ is_txnlog txnlog gid γ.
-
   Definition is_replica_idx (rp : loc) γ α : iProp Σ :=
     ∃ (idx : loc),
       "#HidxP" ∷ readonly (rp ↦[Replica :: "idx"] #idx) ∗
@@ -145,18 +141,31 @@ Section repr.
     ∃ (mu : loc) α,
       "#HmuP"    ∷ readonly (rp ↦[Replica :: "mu"] #mu) ∗
       "#Hlock"   ∷ is_lock tulipNS #mu (own_replica rp gid rid γ α) ∗
-      "#Htxnlog" ∷ is_replica_txnlog rp gid γ ∗
       "#Hidx"    ∷ is_replica_idx rp γ α ∗
       "#Hinv"    ∷ know_tulip_inv γ ∗
       "%Hgid"    ∷ ⌜gid ∈ gids_all⌝ ∗
       "%Hrid"    ∷ ⌜rid ∈ rids_all⌝.
+
+End repr.
+
+Section repr.
+  Context `{!heapGS Σ, !tulip_ghostG Σ, !paxos_ghostG Σ}.
+
+  Definition is_replica_txnlog (rp : loc) gid γ : iProp Σ :=
+    ∃ (txnlog : loc),
+      "#HtxnlogP" ∷ readonly (rp ↦[Replica :: "txnlog"] #txnlog) ∗
+      "#Htxnlog"  ∷ is_txnlog txnlog gid γ.
+
+  Definition is_replica_plus_txnlog (rp : loc) gid rid γ : iProp Σ :=
+    "#Hrp"     ∷ is_replica rp gid rid γ ∗
+    "#Htxnlog" ∷ is_replica_txnlog rp gid γ.
 
   Definition is_replica_plus_network (rp : loc) (addr : chan) (gid rid : u64) γ : iProp Σ :=
     ∃ (addrm : gmap u64 chan),
       "#HaddrP"  ∷ readonly (rp ↦[Replica :: "addr"] (to_val addr)) ∗
       "#HridP"   ∷ readonly (rp ↦[Replica :: "rid"] #rid) ∗
       "#Hinvnet" ∷ know_tulip_network_inv γ gid addrm ∗
-      "Hrp"      ∷ is_replica rp gid rid γ ∗
+      "Hrp"      ∷ is_replica_plus_txnlog rp gid rid γ ∗
       "%Haddr"   ∷ ⌜addrm !! rid = Some addr⌝.
 
 End repr.
