src/program_proof/tulip/program/txnlog/txnlog.v
@@ -1,66 +1,400 @@
+From Perennial.program_proof Require Import marshal_stateless_proof.
 From Perennial.program_proof.tulip.program Require Import prelude.
+From Perennial.program_proof.tulip.program.util Require Import
+  decode_kvmap_into_slice encode_kvmap_from_slice.
+From Perennial.program_proof.tulip.paxos Require Import prelude.
+From Perennial.program_proof.tulip.paxos.program Require Import
+  repr paxos_lookup paxos_submit paxos_wait_until_safe start.
+
+Opaque u64_le.
 
 Section program.
-  Context `{!heapGS Σ, !tulip_ghostG Σ}.
+  Context `{!heapGS Σ, !tulip_ghostG Σ, !paxos_ghostG Σ}.
 
-  Definition is_txnlog (txnlog : loc) (gid : u64) (γ : tulip_names) : iProp Σ.
-  Admitted.
-
-  #[global]
-  Instance is_txnlog_persistent txnlog gid γ :
-    Persistent (is_txnlog txnlog gid γ).
-  Admitted.
+  (*@ type TxnLog struct {                                                    @*)
+  (*@     px *paxos.Paxos                                                     @*)
+  (*@ }                                                                       @*)  
+  Definition is_txnlog (txnlog : loc) (gid : u64) γ : iProp Σ :=
+    ∃ (px : loc) nid π,
+      "#HpxP" ∷ readonly (txnlog ↦[TxnLog :: "px"] #px) ∗
+      "#Hpx"  ∷ is_paxos px nid π ∗
+      "#Hinv" ∷ know_tulip_txnlog_inv γ π gid.
 
   Theorem wp_TxnLog__Lookup (log : loc) (lsn : u64) (gid : u64) γ :
     is_txnlog log gid γ -∗
     {{{ True }}}
-    <<< ∀∀ l, own_txn_log γ gid l >>>
-      TxnLog__Lookup #log #lsn @ ↑txnlogN
-    <<< ∃∃ l', own_txn_log γ gid l' >>>
-    {{{ (c : ccommand) (ok : bool) (pwrsS : Slice.t), RET (ccommand_to_val pwrsS c, #ok);
-        own_pwrs_slice pwrsS c ∗
+    <<< ∀∀ l, own_txn_log_half γ gid l >>>
+      TxnLog__Lookup #log #lsn @ ↑paxosNS ∪ ↑txnlogNS
+    <<< ∃∃ l', own_txn_log_half γ gid l' >>>
+    {{{ (c : ccommand) (ok : bool) (pwrsP : Slice.t), RET (ccommand_to_val pwrsP c, #ok);
+        (if ok then own_pwrs_slice pwrsP c else True) ∗
         ⌜if ok then l' !! (uint.nat lsn) = Some c else True⌝
     }}}.
   Proof.
-  Admitted.
+    iIntros "#Htxnlog" (Φ) "!> _ HAU".
+    wp_rec.
+
+    (*@ func (log *TxnLog) Lookup(lsn uint64) (Cmd, bool) {                     @*)
+    (*@     s, ok := log.px.Lookup(lsn)                                         @*)
+    (*@                                                                         @*)
+    iNamed "Htxnlog".
+    wp_loadField.
+    wp_apply (wp_Paxos__Lookup with "Hpx").
+    iInv "Hinv" as "> HinvO" "HinvC".
+    rewrite difference_difference_l_L.
+    iMod "HAU" as (tlogX) "[HtlogX HAU]".
+    iModIntro.
+    iNamed "HinvO".
+    (* Witness a lower bound of the paxos log. *)
+    iDestruct (log_witness with "Hplog") as "#Hploglb".
+    (* Pass the paxos log to the paxos library. *)
+    iFrame "Hplog".
+    (* Get back the updated paxos log. *)
+    iIntros (plog') "Hplog".
+    (* Derive inclusion property between paxos log and cpool. *)
+    iDestruct (log_cpool_subsume with "Hplog Hpcpool") as %Hincl.
+    (* Prove that the new paxos log is an extension of the old one. *)
+    iDestruct (log_prefix with "Hplog Hploglb") as %Hprefix.
+    destruct Hprefix as [plogext Hplog].
+    (* Assert the existence of the corresponding extension for the txn log. *)
+    assert (∃ tlogext, Forall2 (λ pc tc, tc ∈ tcpool ∧ encode_ccommand tc pc) plogext tlogext)
+      as [tlogext Hext].
+    { apply Forall_exists_Forall2.
+      rewrite Forall_forall.
+      intros x Hx.
+      rewrite /cpool_subsume_log Forall_forall in Hincl.
+      assert (Hin : x ∈ plog') by set_solver.
+      specialize (Hincl _ Hin).
+      specialize (Hcpoolabs _ Hincl). simpl in Hcpoolabs.
+      destruct Hcpoolabs as (tc & Htc & Henc).
+      by exists tc.
+    }
+    (* Agreement of txn log. *)
+    iDestruct (txn_log_agree with "Htlog HtlogX") as %->.
+    (* Update the txn log. *)
+    iMod (txn_log_extend tlogext with "Htlog HtlogX Htcpool")
+      as "(Htlog & HtlogX & Htcpool)".
+    { rewrite /txn_cpool_subsume_log Forall_forall.
+      intros x Hx.
+      rewrite Forall2_lookup in Hext.
+      apply elem_of_list_lookup in Hx as [i Hx].
+      specialize (Hext i).
+      rewrite Hx in Hext.
+      destruct (plogext !! i) as [y |]; last inv Hext.
+      inv Hext.
+      by destruct H1 as [? _].
+    }
+    (* Apply the view shift. *)
+    iMod ("HAU" with "HtlogX") as "HΦ".
+    (* Re-establish the txnlog invariant. *)
+    set tlog' := tlog ++ tlogext.
+    assert (Hlogabs' : Forall2 (λ tc pc, encode_ccommand tc pc) tlog' plog').
+    { rewrite Hplog.
+      apply Forall2_app; first apply Hlogabs.
+      rewrite Forall2_flip.
+      apply (Forall2_impl _ _ _ _ Hext).
+      by intros ? ? [_ ?].
+    }
+    iMod ("HinvC" with "[-HΦ]") as "_".
+    { iFrame.
+      iPureIntro.
+      split; [apply Hlogabs' | apply Hcpoolabs].
+    }
+    iModIntro.
+    iIntros (s ok Hlookup).
+
+    (*@     if !ok {                                                            @*)
+    (*@         return Cmd{}, false                                             @*)
+    (*@     }                                                                   @*)
+    (*@                                                                         @*)
+    wp_pures.
+    destruct ok; wp_pures; last first.
+    { iSpecialize ("HΦ" $! (CmdAbort O) _ Slice.nil).
+      simpl.
+      replace (W64 O) with (W64 0) by word.
+      by iApply "HΦ".
+    }
+
+    (*@     bs := []byte(s)                                                     @*)
+    (*@     kind, bs1 := marshal.ReadInt(bs)                                    @*)
+    (*@                                                                         @*)
+    wp_apply wp_StringToBytes.
+    iIntros (bsP) "Hbs".
+    pose proof (Forall2_lookup_r _ _ _ _ _ Hlogabs' Hlookup)
+      as (tc & Htclookup & Htcenc).
+    destruct tc.
+    {
+      (*@     if kind == TXNLOG_COMMIT {                                          @*)
+      (*@         ts, bs2 := marshal.ReadInt(bs1)                                 @*)
+      (*@         pwrs, _ := util.DecodeKVMapIntoSlice(bs2)                       @*)
+      (*@         cmd := Cmd{                                                     @*)
+      (*@             Kind          : TXNLOG_COMMIT,                              @*)
+      (*@             Timestamp     : ts,                                         @*)
+      (*@             PartialWrites : pwrs,                                       @*)
+      (*@         }                                                               @*)
+      (*@         return cmd, true                                                @*)
+      (*@     }                                                                   @*)
+      (*@                                                                         @*)
+      simpl in Htcenc.
+      destruct Htcenc as (cmddata & Hdata & Hdataenc).
+      rewrite Hdata.
+      iDestruct (own_slice_to_small with "Hbs") as "Hbs".
+      wp_apply (wp_ReadInt with "Hbs").
+      iIntros (p1) "Hbs".
+      wp_pures.
+      destruct Hdataenc as (mdata & Hcmddata & Hmdataenc).
+      rewrite Hcmddata.
+      wp_apply (wp_ReadInt with "Hbs").
+      iIntros (p2) "Hbs".
+      rewrite -(app_nil_r mdata).
+      wp_apply (wp_DecodeKVMapIntoSlice with "Hbs").
+      { apply Hmdataenc. }
+      iIntros (pwrsP dataP) "[Hpwrs Hdata]".
+      wp_pures.
+      iSpecialize ("HΦ" $! (CmdCommit tid pwrs)).
+      iApply "HΦ".
+      by iFrame.
+    }
+    {
+      (*@     if kind == TXNLOG_ABORT {                                           @*)
+      (*@         ts, _ := marshal.ReadInt(bs1)                                   @*)
+      (*@         cmd := Cmd{                                                     @*)
+      (*@             Kind      : TXNLOG_ABORT,                                   @*)
+      (*@             Timestamp : ts,                                             @*)
+      (*@         }                                                               @*)
+      (*@         return cmd, true                                                @*)
+      (*@     }                                                                   @*)
+      (*@                                                                         @*)
+      rewrite Htcenc.
+      iDestruct (own_slice_to_small with "Hbs") as "Hbs".
+      wp_apply (wp_ReadInt with "Hbs").
+      iIntros (p1) "Hbs".
+      wp_pures.
+      wp_apply (wp_ReadInt with "Hbs").
+      iIntros (p2) "Hbs".
+      wp_pures.
+      iSpecialize ("HΦ" $! (CmdAbort tid) _ Slice.nil).
+      iApply "HΦ".
+      by iFrame.
+    }
+
+    (*@     return Cmd{}, false                                                 @*)
+    (*@ }                                                                       @*)
+  Qed.
 
   Theorem wp_TxnLog__SubmitAbort (log : loc) (ts : u64) (gid : u64) γ :
     is_txnlog log gid γ -∗
     {{{ True }}}
-    <<< ∀∀ vs, own_txn_cpool γ gid vs >>>
-      TxnLog__SubmitAbort #log #ts @ ↑txnlogN
-    <<< own_txn_cpool γ gid ({[CmdAbort (uint.nat ts)]} ∪ vs) >>>
-    {{{ (lsn : u64) (term : u64), RET (#lsn, #term);
-        is_proposed_txn_cmd γ gid (uint.nat lsn) (uint.nat term) (CmdAbort (uint.nat ts))
-    }}}.
+    <<< ∀∀ vs, own_txn_cpool_half γ gid vs >>>
+      TxnLog__SubmitAbort #log #ts @ ↑paxosNS ∪ ↑txnlogNS
+    <<< own_txn_cpool_half γ gid ({[CmdAbort (uint.nat ts)]} ∪ vs) >>>
+    {{{ (lsn : u64) (term : u64), RET (#lsn, #term); True }}}.
   Proof.
-  Admitted.
+    iIntros "#Htxnlog" (Φ) "!> _ HAU".
+    wp_rec.
+
+    (*@ func (log *TxnLog) SubmitAbort(ts uint64) (uint64, uint64) {            @*)
+    (*@     bs := make([]byte, 0, 32)                                           @*)
+    (*@     bs1 := marshal.WriteInt(bs, TXNLOG_ABORT)                           @*)
+    (*@     data := marshal.WriteInt(bs1, ts)                                   @*)
+    (*@                                                                         @*)
+    wp_apply wp_NewSliceWithCap; first word.
+    iIntros (p) "Hbs".
+    wp_apply (wp_WriteInt with "Hbs").
+    iIntros (p1) "Hbs".
+    wp_apply (wp_WriteInt with "Hbs").
+    iIntros (p2) "Hbs".
+
+    (*@     lsn, term := log.px.Submit(string(data))                            @*)
+    (*@                                                                         @*)
+    iNamed "Htxnlog".
+    iDestruct (own_slice_to_small with "Hbs") as "Hbs".
+    rewrite uint_nat_W64_0 replicate_0 app_nil_l.
+    wp_apply (wp_StringFromBytes with "Hbs").
+    iIntros "Hbs".
+    wp_loadField.
+    wp_apply (wp_Paxos__Submit with "Hpx").
+    iInv "Hinv" as "> HinvO" "HinvC".
+    rewrite difference_difference_l_L.
+    iMod "HAU" as (tcpoolX) "[HtcpoolX HAU]".
+    iModIntro.
+    iNamed "HinvO".
+    (* Pass the paxos cpool to the paxos library. *)
+    iFrame "Hpcpool".
+    (* Get back the updated paxos cpool. *)
+    iIntros "Hpcpool".
+    (* Agreement of txn cpool. *)
+    iDestruct (txn_cpool_agree with "Htcpool HtcpoolX") as %->.
+    (* Update the txn cpool. *)
+    set tcpool' := _ ∪ tcpool.
+    iMod (txn_cpool_update tcpool' with "Htcpool HtcpoolX") as "[Htcpool HtcpoolX]".
+    { set_solver. }
+    (* Apply the view shift. *)
+    iMod ("HAU" with "HtcpoolX") as "HΦ".
+    (* Re-establish the txnlog invariant. *)
+    iMod ("HinvC" with "[-HΦ]") as "_".
+    { iFrame.
+      iPureIntro.
+      split; first done.
+      apply set_Forall_union; last first.
+      { apply (set_Forall_impl _ _ _ Hcpoolabs).
+        intros x (tc & Htc & Henc).
+        exists tc.
+        split; [set_solver | done].
+      }
+      apply set_Forall_singleton.
+      exists (CmdAbort (uint.nat ts)).
+      split; first set_solver.
+      simpl.
+      rewrite bytes_to_string_to_bytes.
+      rewrite /encode_abort_cmd.
+      by rewrite w64_to_nat_id.
+    }
+    iIntros "!>" (lsn term) "_".
+    wp_pures.
+
+    (*@     return lsn, term                                                    @*)
+    (*@ }                                                                       @*)
+    by iApply "HΦ".
+  Qed.
 
   Theorem wp_TxnLog__SubmitCommit
     (log : loc) (ts : u64) (pwrsS : Slice.t) (pwrs : dbmap) (gid : u64) γ :
     is_txnlog log gid γ -∗
     {{{ own_dbmap_in_slice pwrsS pwrs }}}
-    <<< ∀∀ vs, own_txn_cpool γ gid vs >>>
-      TxnLog__SubmitCommit #log #ts (to_val pwrsS) @ ↑txnlogN
-    <<< own_txn_cpool γ gid ({[CmdCommit (uint.nat ts) pwrs]} ∪ vs) >>>
-    {{{ (lsn : u64) (term : u64), RET (#lsn, #term);
-        is_proposed_txn_cmd γ gid (uint.nat lsn) (uint.nat term) (CmdCommit (uint.nat ts) pwrs)
-    }}}.
+    <<< ∀∀ vs, own_txn_cpool_half γ gid vs >>>
+      TxnLog__SubmitCommit #log #ts (to_val pwrsS) @ ↑paxosNS ∪ ↑txnlogNS
+    <<< own_txn_cpool_half γ gid ({[CmdCommit (uint.nat ts) pwrs]} ∪ vs) >>>
+    {{{ (lsn : u64) (term : u64), RET (#lsn, #term); True }}}.
   Proof.
-  Admitted.
+    iIntros "#Htxnlog" (Φ) "!> Hpwrs HAU".
+    wp_rec.
+
+    (*@ func (log *TxnLog) SubmitCommit(ts uint64, pwrs []tulip.WriteEntry) (uint64, uint64) { @*)
+    (*@     bs := make([]byte, 0, 32)                                           @*)
+    (*@     bs1 := marshal.WriteInt(bs, TXNLOG_COMMIT)                          @*)
+    (*@     bs2 := marshal.WriteInt(bs1, ts)                                    @*)
+    (*@     data := util.EncodeKVMapFromSlice(bs2, pwrs)                        @*)
+    (*@                                                                         @*)
+    wp_apply wp_NewSliceWithCap; first word.
+    iIntros (p) "Hbs".
+    wp_apply (wp_WriteInt with "Hbs").
+    iIntros (p1) "Hbs".
+    wp_apply (wp_WriteInt with "Hbs").
+    iIntros (p2) "Hbs".
+    wp_apply (wp_EncodeKVMapFromSlice with "[$Hbs $Hpwrs]").
+    iIntros (dataP mdata) "(Hbs & Hpwrs & %Hpwrsenc)".
+
+    (*@     lsn, term := log.px.Submit(string(data))                            @*)
+    (*@                                                                         @*)
+    iNamed "Htxnlog".
+    iDestruct (own_slice_to_small with "Hbs") as "Hbs".
+    rewrite uint_nat_W64_0 replicate_0 app_nil_l.
+    wp_apply (wp_StringFromBytes with "Hbs").
+    iIntros "Hbs".
+    wp_loadField.
+    wp_apply (wp_Paxos__Submit with "Hpx").
+    iInv "Hinv" as "> HinvO" "HinvC".
+    rewrite difference_difference_l_L.
+    iMod "HAU" as (tcpoolX) "[HtcpoolX HAU]".
+    iModIntro.
+    iNamed "HinvO".
+    (* Pass the paxos cpool to the paxos library. *)
+    iFrame "Hpcpool".
+    (* Get back the updated paxos cpool. *)
+    iIntros "Hpcpool".
+    (* Agreement of txn cpool. *)
+    iDestruct (txn_cpool_agree with "Htcpool HtcpoolX") as %->.
+    (* Update the txn cpool. *)
+    set tcpool' := _ ∪ tcpool.
+    iMod (txn_cpool_update tcpool' with "Htcpool HtcpoolX") as "[Htcpool HtcpoolX]".
+    { set_solver. }
+    (* Apply the view shift. *)
+    iMod ("HAU" with "HtcpoolX") as "HΦ".
+    (* Re-establish the txnlog invariant. *)
+    iMod ("HinvC" with "[-HΦ]") as "_".
+    { iFrame.
+      iPureIntro.
+      split; first done.
+      apply set_Forall_union; last first.
+      { apply (set_Forall_impl _ _ _ Hcpoolabs).
+        intros x (tc & Htc & Henc).
+        exists tc.
+        split; [set_solver | done].
+      }
+      apply set_Forall_singleton.
+      exists (CmdCommit (uint.nat ts) pwrs).
+      split; first set_solver.
+      rewrite /= bytes_to_string_to_bytes -app_assoc.
+      exists (u64_le ts ++ mdata).
+      split; first done.
+      exists mdata.
+      split; last done.
+      by rewrite w64_to_nat_id.
+    }
+    iIntros "!>" (lsn term) "_".
+    wp_pures.
+
+    (*@     return lsn, term                                                    @*)
+    (*@ }                                                                       @*)
+    by iApply "HΦ".
+  Qed.
 
   Theorem wp_TxnLog__WaitUntilSafe
-    (log : loc) (lsn : u64) (term : u64) (c : ccommand) (gid : u64) γ :
+    (log : loc) (lsn : u64) (term : u64) (gid : u64) γ :
     is_txnlog log gid γ -∗
-    is_proposed_txn_cmd γ gid (uint.nat lsn) (uint.nat term) c -∗
     {{{ True }}}
       TxnLog__WaitUntilSafe #log #lsn #term
-    {{{ (ok : bool), RET #ok;
-        if ok
-        then ∃ l, is_txn_log_lb γ gid l ∧ ⌜l !! (uint.nat lsn) = Some c⌝
-        else True
-    }}}.
+    {{{ (ok : bool), RET #ok; True }}}.
   Proof.
-  Admitted.
+    iIntros "#Htxnlog" (Φ) "!> _ HΦ".
+    wp_rec.
+
+    (*@ func (log *TxnLog) WaitUntilSafe(lsn uint64, term uint64) bool {        @*)
+    (*@     return log.px.WaitUntilSafe(lsn, term)                              @*)
+    (*@ }                                                                       @*)
+    iNamed "Htxnlog".
+    wp_loadField.
+    by wp_apply (wp_Paxos__WaitUntilSafe with "Hpx").
+  Qed.
+
+  Theorem wp_Start
+    (nidme : u64) (termc : u64) (terml : u64) (lsnc : u64) (log : list string)
+    (addrmP : loc) (addrm : gmap u64 chan) (fname : string) gid γ π :
+    is_node_wal_fname π nidme fname -∗
+    know_paxos_inv π (dom addrm) -∗
+    know_paxos_file_inv π (dom addrm) -∗
+    know_paxos_network_inv π addrm -∗
+    know_tulip_txnlog_inv γ π gid -∗
+    {{{ own_map addrmP (DfracOwn 1) addrm ∗
+        own_current_term_half π nidme (uint.nat termc) ∗
+        own_ledger_term_half π nidme (uint.nat terml) ∗
+        own_committed_lsn_half π nidme (uint.nat lsnc) ∗
+        own_node_ledger_half π nidme log
+    }}}
+      Start #nidme #addrmP #(LitString fname)
+    {{{ (txnlog : loc), RET #txnlog; is_txnlog txnlog gid γ }}}.
+  Proof.
+    iIntros "#Hfnamewal #Hinv #Hinvfile #Hinvnet #Hinvtxnlog" (Φ).
+    iIntros "!> (Haddrm & Htermc & Hterml & Hlsnc & Hlogn) HΦ".
+    wp_rec. wp_pures.
+
+    (*@ func Start(nidme uint64, addrm map[uint64]grove_ffi.Address, fname string) *TxnLog { @*)
+    (*@     px := paxos.Start(nidme, addrm, fname)                              @*)
+    (*@     txnlog := &TxnLog{ px : px }                                        @*)
+    (*@     return txnlog                                                       @*)
+    (*@ }                                                                       @*)
+    wp_apply (wp_Start
+               with "Hfnamewal Hinv Hinvfile Hinvnet [$Haddrm $Htermc $Hterml $Hlsnc $Hlogn]").
+    iIntros (pxP) "#Hpx".
+    wp_apply (wp_allocStruct); first by auto.
+    iIntros (txnlogP) "HtxnlogP".
+    iDestruct (struct_fields_split with "HtxnlogP") as "HtxnlogP".
+    iNamed "HtxnlogP".
+    wp_pures.
+    iMod (readonly_alloc_1 with "px") as "#HpxP".
+    iApply "HΦ".
+    by iFrame "#".
+  Qed.
 
 End program.
